Heap interface: Support reasoning about freshness.

theories/heap_lang/heap.v
@@ -1,5 +1,5 @@
 From iris.prelude Require Import gmultiset.
-From iris.algebra Require Import auth gmap csum agree.
+From iris.algebra Require Import auth gmap coPset csum agree.
 From iris.algebra Require Export gset frac.
 From iris.base_logic.lib Require Export invariants.
 From iris.base_logic.lib Require Import own auth fractional.
@@ -10,26 +10,29 @@ From iris.proofmode Require Import tactics.
 Import uPred.
 Import addenda.fin_maps.
 Import addenda.option addenda.gmap addenda.csum.
-Import addenda.lib_auth.
+Import addenda.lib_auth addenda.algebra_auth.
 
 Local Hint Resolve to_of_val.
 
-(** The CMRA we need. *)
+(** The CMRAs we need. *)
 Local Notation heap := (gmap loc val).
 Definition heapN : namespace := nroot .@ "heap".
 Definition heapUR : ucmraT :=
   gmapUR loc (csumR (prodR fracR (agreeR valC)) unitR).
 Local Notation Hval q v := (Cinl (q%Qp, to_agree v)).
 Local Notation Lval := (Cinr ()).
+Local Notation locset := (gsetUR loc).
 
 Class heapG Σ := HeapG {
   heap_ownP_inG :> ownPG heap_lang Σ;
+  heap_liveG_inG :> inG Σ (authR locset);
   heap_inG :> authG Σ heapUR;
-  heap_name : gname
+  heap_name : gname * gname
 }.
 
 Class heapPreG Σ := HeapPreG {
   heap_preG_ownP_inG : ownPPreG heap_lang Σ;
+  heap_preG_liveG_inG : inG Σ (authR locset);
   heap_preG_inG : authG Σ heapUR
 }.
 (*
@@ -38,89 +41,106 @@ Class heapPreG Σ := HeapPreG {
  * "inner" [heapG] rather than the "outer" [heapPreG].
  *)
 Existing Instance heap_preG_ownP_inG | 30.
+Existing Instance heap_preG_liveG_inG | 30.
 Existing Instance heap_preG_inG | 30.
 
-Definition heapΣ : gFunctors := #[ownPΣ state; authΣ heapUR].
+Definition heapΣ : gFunctors := #[
+  ownPΣ state; GFunctor (constRF (authR locset)); authΣ heapUR
+].
 Instance subG_heapPreG {Σ} : subG heapΣ Σ → heapPreG Σ.
-Proof. intros [??]%subG_inv; constructor; apply _. Qed.
+Proof. intros [?[??]%subG_inv]%subG_inv. constructor; apply _. Qed.
 
 (** * Heap resources and invariant *)
 Section definitions.
-  Context `{ownPG heap_lang Σ, authG Σ heapUR} (γ : gname).
+  Context `{ownPG heap_lang Σ, inG Σ (authR locset), authG Σ heapUR}.
+  Context (γ : gname * gname).
   Implicit Types l : loc.
   Implicit Types q : Qp.
   Implicit Types v : val.
   Implicit Types h : heap.
 
+  (** Live locations. *)
+  Definition liveloc'_def l : iProp Σ := own (γ.2) (◯ (to_gset {[ l ]})).
+  Definition liveloc'_aux : { x | x = @liveloc'_def }. by eexists. Qed.
+  Definition liveloc' := proj1_sig liveloc'_aux.
+  Definition liveloc'_eq : @liveloc' = @liveloc'_def := proj2_sig liveloc'_aux.
+
   (** High locations. *)
-  Definition mapsto_def l q v : iProp Σ := auth_own γ {[l := Hval q v]}.
+  Definition mapsto_def l q v : iProp Σ :=
+    (auth_own (γ.1) {[l := Hval q v]} ∗ liveloc' l)%I.
   Definition mapsto_aux : { x | x = @mapsto_def }. by eexists. Qed.
   Definition mapsto := proj1_sig mapsto_aux.
   Definition mapsto_eq : @mapsto = @mapsto_def := proj2_sig mapsto_aux.
 
   (** Low locations. *)
-  Definition lowloc'_def l : iProp Σ := auth_own γ {[l := Lval]}.
+  Definition lowloc'_def l : iProp Σ :=
+    (auth_own (γ.1) {[l := Lval]} ∗ liveloc' l)%I.
   Definition lowloc'_aux : { x | x = @lowloc'_def }. by eexists. Qed.
   Definition lowloc' := proj1_sig lowloc'_aux.
   Definition lowloc'_eq : @lowloc' = @lowloc'_def := proj2_sig lowloc'_aux.
 
   (** Low values. *)
-  Notation lowval := (on_val lowloc').
+  Notation lowval' := (on_val lowloc').
 
   (**
     Invariant: The state is good and maps every high location to its
-    value and every low location to a low value.
+    value and every low location to a low value. Locations are live
+    when they're in the heap's domain.
   *)
   Definition to_high : heap → heapUR := fmap (λ v, Hval 1 v).
   Definition to_low : heap → heapUR  := fmap (λ _, Lval).
   Definition to_heap (a : heap * heap) : heapUR :=
     let: (h, h') := a in to_high h ⋅ to_low h'.
-  Definition hinv' (a : heap * heap) : iProp Σ :=
+  Definition hinv' (a : heap * heap) : iProp Σ := (
     let: (h, h') := a in
-    (ownP (good_state (h ∪ h')) ∗ [∗ map] v ∈ h', lowval v)%I.
+    ownP (good_state (h ∪ h'))
+    ∗ ([∗ map] v ∈ h', lowval' v)
+    ∗ own (γ.2) (● (dom (gset loc) (h ∪ h')))
+  )%I.
 
-  Lemma hinv_alloc h : ownP (good_state h) -∗ ▷ hinv' (h, ∅).
+  Lemma hinv_alloc h :
+    ownP (good_state h) ∗ own (γ.2) (● dom (gset loc) h) ⊢ ▷ hinv' (h, ∅).
   Proof.
-    rewrite /hinv' right_id big_sepM_empty right_id. exact: later_intro.
+    rewrite /hinv' right_id big_sepM_empty left_id. exact: later_intro.
   Qed.
 
   Lemma to_heap_valid h : ✓ to_heap (h, ∅).
   Proof. move=>l. rewrite lookup_op !lookup_fmap. by case (h !! l). Qed.
 
-  Definition heap_ctx' : iProp Σ := auth_ctx γ heapN to_heap hinv'.
-  Global Instance heap_ctx_persistent : PersistentP heap_ctx'.
+  Definition heap_ctx' : iProp Σ := auth_ctx (γ.1) heapN to_heap hinv'.
+
+  Global Instance heap_ctx'_persistent : PersistentP heap_ctx'.
   Proof. apply _. Qed.
 End definitions.
-Typeclasses Opaque mapsto lowloc'.
-(* PDS: heap_ctx' not opaque because we lack some instances. *)
-Instance: Params (@mapsto) 2.
-Instance: Params (@lowloc') 2.
-Instance: Params (@heap_ctx') 3.
+
+Notation liveloc := (liveloc' heap_name).
 
 Notation "l ↦{ q } v" := (mapsto heap_name l q v)
   (at level 20, q at level 50, format "l  ↦{ q }  v") : uPred_scope.
 Notation "l ↦ v" := (mapsto heap_name l 1 v) (at level 20) : uPred_scope.
-
 Notation "l ↦{ q } -" := (∃ v, l ↦{q} v)%I
   (at level 20, q at level 50, format "l  ↦{ q }  -") : uPred_scope.
 Notation "l ↦ -" := (l ↦{1} -)%I (at level 20) : uPred_scope.
 
 Notation lowloc := (lowloc' heap_name).
+Notation lowval := (on_val lowloc).
 Notation heap_ctx := (heap_ctx' heap_name).
 Local Notation hinv := (hinv' heap_name).
 
 (** Allocating the invariant. *)
-(** We cannot use [auth_alloc] as [hinv] depends on the ghost name. *)
-Lemma heap_ctx_alloc `{ownPG heap_lang Σ, authG Σ heapUR} E h :
+(** We cannot use [auth_alloc] as [hinv] depends on the ghost names. *)
+Lemma heap_ctx_alloc `{ownPG heap_lang Σ, inG Σ (authR locset), authG Σ heapUR} E h :
   ownP (good_state h) ={E}=∗ ∃ γ, heap_ctx' γ.
 Proof.
-  iIntros "Hσ". set h' := to_heap (h, ∅).
-  iMod (own_alloc (Auth (Excl' h') h')) as (γ) "Ha".
+  iIntros "Hσ". set h' := to_heap (h, ∅). set X := dom (gset loc) h.
+  iMod (own_alloc (Auth (Excl' h') h')) as (γheap) "Ha".
   { split. done. exact: to_heap_valid. }
-  set hinv_γ := @hinv' _ _ _ γ.
-  iRevert "Ha"; rewrite auth_both_op; iIntros "[Ha _]".
-  iDestruct (@hinv_alloc _ _ _ γ with "Hσ") as "Hσ".
-  iMod (inv_alloc heapN _ (auth_inv γ to_heap hinv_γ) with "[Ha Hσ]") as "#?".
+  iMod (own_alloc (Auth (Excl' X) X)) as (γlive) "Hlive"; first done.
+  set γ := (γheap, γlive). set hinv_γ := @hinv' _ _ _ _ γ.
+  rewrite (auth_both_op h') (auth_both_op X).
+  iDestruct "Ha" as "[Ha _]". iDestruct "Hlive" as "[Hlive _]".
+  iDestruct (@hinv_alloc _ _ _ _ γ with "[$Hσ $Hlive]") as "Hh".
+  iMod (inv_alloc heapN _ (auth_inv γheap to_heap hinv_γ) with "[-]") as "#?".
   { iNext. rewrite/auth_inv. iExists (h, ∅). by iFrame. }
   iModIntro. iExists γ. by rewrite/heap_ctx'/auth_ctx.
 Qed.
@@ -129,12 +149,35 @@ Qed.
 Lemma heap_ctx_is_good `{heapG Σ} E :
  ↑heapN ⊆ E → heap_ctx ={E,∅}=∗ ∃ σ, ownP σ ∧ ⌜is_good σ⌝.
 Proof.
-  iIntros (?) "Hinv". iMod (fupd_intro_mask' _ (↑heapN)) as "_"; first done.
-  iMod (auth_empty heap_name) as "Ha".
-  iMod (auth_open with "[$Hinv $Ha]") as ([h h']) "(_&[>Hh _]&_)";
+  iIntros (?) "Hh". iMod (fupd_intro_mask' _ (↑heapN)) as "_"; first done.
+  iMod (auth_empty (heap_name.1)) as "Ha".
+  iMod (auth_open with "[$Hh $Ha]") as ([h h']) "(_&[>Hh _]&_)";
     first done.
   iExists _; iFrame. by rewrite subseteq_empty_difference_L.
 Qed.
+
+(** Live locations *)
+Section live.
+  Context `{heapG Σ}.
+
+  Definition live : gset loc → iProp Σ := λ X, ([∗ set] l ∈ X, liveloc l)%I.
+
+  Global Instance liveloc_persistent l : PersistentP (liveloc l).
+  Proof. rewrite liveloc'_eq. apply _. Qed.
+  Global Instance liveloc_timeless l : TimelessP (liveloc l).
+  Proof. rewrite liveloc'_eq. apply _. Qed.
+
+  Global Instance live_persistent X : PersistentP (live X).
+  Proof. apply _. Qed.
+  Global Instance live_timeless X : TimelessP (live X).
+  Proof. apply _. Qed.
+
+  Lemma lowloc_live l : lowloc l ⊢ liveloc l.
+  Proof. by rewrite lowloc'_eq /lowloc'_def sep_elim_r. Qed.
+
+  Lemma mapsto_live l q v : l ↦{q} v ⊢ liveloc l.
+  Proof. by rewrite mapsto_eq /mapsto_def sep_elim_r. Qed.
+End live.
 
 (** * Low integrity predicates *)
 Class LowIntegrity Σ (A : Type) := Low {
@@ -157,15 +200,20 @@ Section low.
     (irreversible) ghost move [heap_mark_low].
   *)
   Global Instance lowloc_persistent l : PersistentP (lowloc l).
-  Proof. rewrite lowloc'_eq /lowloc'_def. apply _. Qed.
+  Proof. rewrite lowloc'_eq. apply _. Qed.
+  Global Instance lowloc_timeless l : TimelessP (lowloc l).
+  Proof. rewrite lowloc'_eq. apply _. Qed.
   Global Instance loc_low : LowIntegrity Σ loc := Low lowloc _ _.
   Global Instance loc_low_timeless (l : loc) : TimelessP (low l).
-  Proof. rewrite /low/= lowloc'_eq /lowloc'_def. apply _. Qed.
+  Proof. rewrite /low/=. apply _. Qed.
 
   Lemma low_loc l : low l ⊣⊢ lowloc l. Proof. by []. Qed.
 
+  Lemma low_live l : low l ⊢ liveloc l.
+  Proof. by rewrite low_loc lowloc_live. Qed.
+
   (** Low values lift low locations to values. *)
-  Global Instance val_low : LowIntegrity Σ val := Low (on_val lowloc) _ _.
+  Global Instance val_low : LowIntegrity Σ val := Low lowval _ _.
 
   Lemma low_val_eq v : low v ⊣⊢ on_val lowloc v. Proof. by []. Qed.
 
@@ -213,7 +261,16 @@ Ltac simpl_low :=
 Local Hint Extern 5 => simpl_low.
 
 (** * Bookkeeping lemmas *)
-Section bookkeeping.
+Module internal.
+
+Notation Live h := (own (heap_name.2) (● dom (gset loc) h)) (only parsing).
+Notation HighLoc l q v := (auth_own (heap_name.1) {[l := Hval q v]})
+  (only parsing).
+Notation LowLoc l := (auth_own (heap_name.1) {[l := Lval ]}) (only parsing).
+Notation Phys h := (ownP (good_state h)) (only parsing).
+Notation Low h' := ([∗ map] v' ∈ h', low v')%I (only parsing).
+
+Section internal.
   Context `{heapG Σ}.
   Implicit Types l : loc.
   Implicit Types q : Qp.
@@ -345,6 +402,73 @@ Section bookkeeping.
     apply lookup_to_heap_None, lookup_union_None. by rewrite lookup_delete.
   Qed.
 
+  Lemma high_eq l q v : l ↦{q} v ⊣⊢ HighLoc l q v ∗ liveloc l.
+  Proof. by rewrite mapsto_eq. Qed.
+
+  Lemma high_HighLoc l q v : l ↦{q} v ⊢ HighLoc l q v.
+  Proof. by rewrite high_eq sep_elim_l. Qed.
+
+  Lemma low_eq l : low l ⊣⊢ LowLoc l ∗ liveloc l.
+  Proof. by rewrite low_loc lowloc'_eq. Qed.
+
+  Lemma hinv_mark_low h h' l v :
+    ✓ to_heap (h, h') → {[l := Hval 1 v]} ≼ to_heap (h, h') →
+    ▷ low v -∗ ▷ Phys (h ∪ h') -∗ ▷ Low h' -∗ ▷ Live (h ∪ h') -∗
+    ▷ hinv (delete l h, <[l:=v]> h').
+  Proof.
+    move=>Hv /to_heap_high_included -/(_ Hv)[??]. rewrite/hinv.
+    iIntros "Hv Hσ Hlow Hlive". rewrite -delete_insert_union //.
+    iFrame. rewrite 2!big_sepM_later big_sepM_insert //. by iFrame.
+  Qed.
+
+  (* PDS: Hoist. *)
+  Lemma to_gset_singleton l : to_gset {[l]} = {[l]}.
+  Proof.
+    apply mapset_eq=> x. rewrite elem_of_to_gset; last exact: singleton_finite.
+    by rewrite 2!elem_of_singleton.
+  Qed.
+
+  Lemma live_obs h l X :
+    h !! l = None →
+    Live h -∗ live X -∗ ⌜l ∉ X⌝.
+  Proof.
+    rewrite/live liveloc'_eq /liveloc'_def=>Hdom.
+    induction X as [|x X Hx IH] using collection_ind_L.
+    { iIntros "Hh _". iPureIntro. exact: not_elem_of_empty. }
+    iIntros "Hh HX".
+    rewrite big_sepS_union; last by move=>?/elem_of_singleton->.
+    rewrite big_sepS_singleton. iDestruct "HX" as "(Hx & HX)".
+    iDestruct (IH with "Hh HX") as "%". rewrite not_elem_of_union.
+    case: (decide (l = x))=>?; last first.
+    { iFrame. iPureIntro. by rewrite not_elem_of_singleton. }
+    subst. iExFalso. iDestruct (own_valid_2 with "Hh Hx") as "Hv".
+    iDestruct "Hv" as %[Hinc%gset_included _]%auth_valid_discrete_2.
+    iPureIntro. move: Hinc=>/(_ x).
+    rewrite (to_gset_singleton x) elem_of_singleton=>
+      /(_ (eq_refl _))/elem_of_dom.
+    by rewrite Hdom=>-[].
+  Qed.
+
+  Lemma live_alloc h l v :
+    Live h ==∗ Live (<[l:=v]> h) ∗ liveloc l.
+  Proof.
+    rewrite/live liveloc'_eq /liveloc'_def.
+    rewrite -(sep_elim_r (own (heap_name.2) (◯ dom (gset loc) h))
+      (own _ (◯ to_gset {[l]}))) -2!own_op -auth_frag_op.
+    apply own_update, auth_update_alloc.
+    rewrite dom_insert comm gset_op_union (to_gset_singleton l).
+    apply gset_local_update, union_subseteq_l.
+  Qed.
+
+  Lemma hinv_high h h' l v :
+    Phys (<[l:=v]> (h ∪ h')) -∗ Low h' -∗ Live (<[l:=v]> (h ∪ h')) -∗
+    hinv (<[l:=v]> h, h').
+  Proof. rewrite/hinv insert_union_l. by iIntros; iFrame. Qed.
+
+  Lemma hinv_intro h h' :
+    Phys (h ∪ h') -∗ Low h' -∗ Live (h ∪ h') -∗ hinv (h, h').
+  Proof. rewrite/hinv. by iIntros; iFrame. Qed.
+
   Lemma to_heap_alloc_high h h' l v :
     (h ∪ h') !! l = None →
     (to_heap (h, h'), ∅) ~l~> (to_heap (<[l:=v]> h, h'), {[l := Hval 1 v]}).
@@ -353,6 +477,16 @@ Section bookkeeping.
     rewrite to_heap_high_insert; last by move: Hdom=>/lookup_union_None[].
     apply alloc_singleton_local_update; last done.
     by apply lookup_to_heap_None.
+  Qed.
+
+  Lemma live_store_high h h' l v' v :
+    h !! l = Some v' → h' !! l = None →
+    Live (h ∪ h') ⊣⊢ Live (<[l:=v]> (h ∪ h')).
+  Proof.
+    move=>??. do 4!f_equiv. apply mapset_eq=>x. rewrite 2!elem_of_dom.
+    case: (decide (x = l))=>?.
+    - subst. simplify_map_eq. by rewrite 2!is_Some_alt.
+    - by rewrite lookup_insert_ne.
   Qed.
 
   Lemma to_heap_store_high h h' l v1 v2 :
@@ -365,35 +499,36 @@ Section bookkeeping.
     exact: exclusive_local_update.
   Qed.
 
-  Lemma hinv_intro h h' :
-    ownP (good_state (h ∪ h')) -∗ ([∗ map] v ∈ h', low v) -∗ hinv (h, h').
-  Proof. rewrite/hinv. by iIntros; iFrame. Qed.
-
-  Lemma hinv_high h h' l v :
-    ownP (good_state (<[l:=v]> (h ∪ h'))) -∗ ([∗ map] v ∈ h', low v) -∗
-    hinv (<[l:=v]> h, h').
-  Proof. rewrite/hinv insert_union_l. by iIntros; iFrame. Qed.
-
-  Lemma hinv_mark_low h h' l v :
-    ✓ to_heap (h, h') → {[l := Hval 1 v]} ≼ to_heap (h, h') →
-    ▷ ownP (good_state (h ∪ h')) -∗
-    ▷ low v -∗ ▷ ([∗ map] v' ∈ h', low v') -∗ ▷ hinv (delete l h, <[l:=v]>h').
+  Lemma live_store_low h h' l v1 v2 :
+    h !! l = None → h' !! l = Some v1 →
+    Live (h ∪ h') ⊣⊢ Live (h ∪ <[l:=v2]> h').
   Proof.
-    move=>Hv /to_heap_high_included -/(_ Hv)[??]. rewrite/hinv.
-    iIntros "Hh Hv Hlow". rewrite -delete_insert_union //.
-    iFrame. rewrite 2!big_sepM_later big_sepM_insert //. by iFrame.
+    move=>Hhigh Hlow.
+    do 4!f_equiv. apply mapset_eq=>x. rewrite 2!elem_of_dom.
+    case: (decide (x = l))=>?.
+    - subst. rewrite (lookup_union_Some_r' _ _ _ v1) //.
+      rewrite (lookup_union_Some_r' _ _ _ v2) //.
+      by rewrite 2!is_Some_alt.  by rewrite lookup_insert.
+    - case Hleft: (h !! x) => [v|]; first by simplify_map_eq.
+      case Hright: (h' !! x) => [v'|].
+      + do 2!rewrite (lookup_union_Some_r' _ _ _ v') //.
+        by rewrite lookup_insert_ne.
+      + have->: (h ∪ h') !! x = None by apply lookup_union_None.
+        have->: (h ∪ <[l:=v2]> h') !! x = None; last done.
+        apply lookup_union_None. by rewrite lookup_insert_ne.
   Qed.
 
   Lemma hinv_store_low h h' l v1 v2 :
     h !! l = None → h' !! l = Some v1 →
-    ownP (good_state (<[l:=v2]> (h ∪ h'))) -∗
-    ([∗ map] v ∈ h', low v) -∗ low v2 -∗ hinv (h, <[l:=v2]> h').
+    low v2 -∗ Phys (<[l:=v2]> (h ∪ h')) -∗ Low h' -∗ Live (h ∪ <[l:=v2]> h') -∗
+    hinv (h, <[l:=v2]> h').
   Proof.
     move=>??.
     rewrite /hinv insert_union_r // big_sepM_insert_override_2 //.
-    iIntros "? Hlow ?". iFrame. iApply "Hlow". eauto.
+    iIntros "? ? Hlow ?". iFrame. iApply "Hlow". eauto.
   Qed.
-End bookkeeping.
+End internal.
+End internal.
 
 (** * Heap interface *)
 Section heap.
@@ -402,22 +537,32 @@ Section heap.
   Implicit Types q : Qp.
   Implicit Types v : val.
   Implicit Types h : heap.
+  Import internal.
 
-  (** High and low locations are disjoint. *)
+  (** ** Structure *)
+  (**
+	High locations and the heap context enjoy their usual
+	properties. Low locations are timeless, persistent, and
+	disjoint from high locations. High locations containing low
+	values can be marked low.
+  *)
   Lemma high_not_low l q v : l ↦{q} v ∗ low l ⊢ False.
   Proof.
-    by rewrite mapsto_eq low_loc lowloc'_eq
-      -auth_own_op auth_own_valid discrete_valid
-      op_singleton singleton_valid.
+    rewrite high_HighLoc low_eq (sep_elim_l _ (liveloc _)).
+    rewrite -auth_own_op auth_own_valid discrete_valid.
+    by rewrite op_singleton singleton_valid.
   Qed.
 
-  (** High locations enjoy their usual properties. *)
   Global Instance mapsto_timeless l q v : TimelessP (l ↦{q} v).
   Proof. rewrite mapsto_eq. apply _. Qed.
   Global Instance mapsto_fractional l v : Fractional (λ q, l ↦{q} v)%I.
   Proof.
-    intros p q. by rewrite mapsto_eq -auth_own_op
-      op_singleton Cinl_op pair_op agree_idemp.
+    enough (F : Fractional (λ q, HighLoc l q v)).
+    { intros p q. rewrite 3!high_eq. iSplit.
+      - iIntros "(Hpq & #HL)". iFrame "HL HL". by rewrite -F.
+      - iIntros "([Hp _] & Hq & HL)". rewrite (F p q). by iFrame "Hp Hq HL". }
+    intros p q. rewrite -auth_own_op.
+    by rewrite op_singleton Cinl_op pair_op agree_idemp.
   Qed.
   Global Instance mapsto_as_fractional l q v :
     AsFractional (l ↦{q} v) (λ q, l ↦{q} v)%I q.
@@ -425,8 +570,8 @@ Section heap.
 
   Lemma mapsto_agree l q1 q2 v1 v2 : l ↦{q1} v1 ∗ l ↦{q2} v2 ⊢ ⌜v1 = v2⌝.
   Proof.
-    rewrite mapsto_eq -auth_own_op auth_own_valid discrete_valid
-      op_singleton singleton_valid Cinl_op pair_op.
+    rewrite 2!high_HighLoc -auth_own_op auth_own_valid.
+    rewrite discrete_valid op_singleton singleton_valid Cinl_op pair_op.
     by f_equiv=> -[] _ /agree_op_inv/to_agree_inj/leibniz_equiv_iff.
   Qed.
 
@@ -443,8 +588,7 @@ Section heap.
 
   Lemma mapsto_valid l q v : l ↦{q} v ⊢ ✓ q.
   Proof.
-    rewrite mapsto_eq /mapsto_def auth_own_valid !discrete_valid
-      singleton_valid.
+    rewrite high_HighLoc auth_own_valid 2!discrete_valid singleton_valid.
     by apply pure_mono=> -[].
   Qed.
   Lemma mapsto_valid_2 l q1 q2 v1 v2 : l ↦{q1} v1 ∗ l ↦{q2} v2 ⊢ ✓ (q1 + q2)%Qp.
@@ -453,46 +597,37 @@ Section heap.
     iApply (mapsto_valid l _ v2). by iFrame.
   Qed.
 
-  (** High locations containing low values may be marked low. *)
   Lemma heap_mark_low E l v :
     ↑heapN ⊆ E →
     heap_ctx -∗ ▷ l ↦ v -∗ ▷ low v ={E}=∗ low l.
   Proof.
-    iIntros (?) "#Hinv >Hl Hv". rewrite /heap_ctx mapsto_eq /mapsto_def.
-    iMod (auth_open_strong with "[$Hinv $Hl]")
-      as ([h h']) "(%&%&[Hh Hlow]&Hcl)"; first done.
-    iDestruct (hinv_mark_low with "Hh Hv Hlow") as "Hh"; [done|done|].
-    iMod ("Hcl" with "* [Hh]") as "Ha".
+    rewrite high_eq. iIntros (?) "Hh >(Hl & HL) Hv".
+    iMod (auth_open_strong with "[$Hh $Hl]")
+      as ([h h']) "(%&%&(Hσ&Hlow&Hlive)&Hcl)"; first done.
+    iDestruct (hinv_mark_low with "Hv Hσ Hlow Hlive") as "Hh"=>//.
+    iMod ("Hcl" with "* [Hh]") as "Hl".
     - iFrame. iPureIntro. exact: to_heap_mark_low.
-    - by rewrite low_loc lowloc'_eq /lowloc'_def.
+    - rewrite low_eq. by iFrame.
   Qed.
 
-  (** Heap rules for high and low locations. *)
-  Lemma wp_alloc p E e v :
+  (** ** Operational rules *)
+
+  Lemma wp_alloc_live p E e v X :
     to_val e = Some v → ↑heapN ⊆ E →
-    {{{ heap_ctx }}} Alloc e @ p; E {{{ l, RET LocV l; l ↦ v }}}.
+    {{{ heap_ctx ∗ live X }}} Alloc e @ p; E
+    {{{ l, RET LocV l; l ↦ v ∗ ⌜l ∉ X⌝ }}}.
   Proof.
-    iIntros (<-%of_to_val ? Φ) "#Hinv HΦ". rewrite /heap_ctx.
-    iMod (auth_empty heap_name) as "Ha".
-    iMod (auth_open with "[$Hinv $Ha]") as ([h h']) "(%&[Hh Hlow]&Hcl)";
-      first done.
-    iApply (wp_alloc_pst with "Hh"); first done. iNext. iIntros (l) "[% Hh]".
-    iDestruct (hinv_high with "Hh Hlow") as "Hh".
-    iMod ("Hcl" with "* [Hh]") as "Ha".
+    iIntros (<-%of_to_val ? Φ) "(Hh&#HX) HΦ". rewrite /heap_ctx.
+    iMod (auth_empty (heap_name.1)) as "Ha".
+    iMod (auth_open with "[$Hh $Ha]")
+      as ([h h']) "(%&(Hσ & Hlow & Hlive)&Hcl)"; first done.
+    iApply (wp_alloc_big with "Hσ"); first done. iNext. iIntros (l) "[% Hσ]".
+    iDestruct (live_obs _ l X with "Hlive HX") as "#HXl"; first done.
+    iMod (live_alloc _ l v with "Hlive") as "(Hlive & HL)".
+    iDestruct (hinv_high with "Hσ Hlow Hlive") as "Hh".
+    iMod ("Hcl" with "* [Hh]") as "Hl".
     - iFrame. iPureIntro. exact: to_heap_alloc_high.
-    - iApply "HΦ". by rewrite mapsto_eq /mapsto_def.
-  Qed.
-
-  Lemma wp_alloc_low p E e v :
-    to_val e = Some v → ↑heapN ⊆ E →
-    {{{ heap_ctx ∗ ▷ low v }}} Alloc e @ p; E
-    {{{ l, RET LocV l; low l }}}.
-  Proof.
-    iIntros (?? Φ) "[#Hinv Hv] HΦ". rewrite -wp_fupd.
-    iApply (wp_alloc with "Hinv"); eauto.
-    iNext. iIntros (l) "Hl". rewrite [(l ↦ v)%I]later_intro [low _]later_intro.
-    iDestruct (heap_mark_low with "Hinv Hl Hv") as "Hl"; first done.
-    by iApply ("HΦ" with "Hl").
+    - iApply "HΦ". rewrite high_eq. by iFrame.
   Qed.
 
   Lemma wp_load p E l q v :
@@ -500,14 +635,14 @@ Section heap.
     {{{ heap_ctx ∗ ▷ l ↦{q} v }}} Load (Loc l) @ p; E
     {{{ RET v; l ↦{q} v }}}.
   Proof.
-    iIntros (? Φ) "[#Hinv >Hl] HΦ".
-    rewrite /heap_ctx mapsto_eq /mapsto_def.
-    iMod (auth_open_strong with "[$Hinv $Hl]")
-      as ([h h']) "(%&%&[Hh Hlow]&Hcl)"; first done.
+    iIntros (? Φ) "[Hh >Hl] HΦ". rewrite high_eq. iDestruct "Hl" as "[Hl HL]".
+    iMod (auth_open_strong with "[$Hh $Hl]")
+      as ([h h']) "(%&%&(Hσ & Hlow & Hlive)&Hcl)"; first done.
     case: (to_heap_high_included h h' l q v) => // ??.
-    iApply (wp_load_pst with "Hh"); [done|exact: lookup_union_Some_l|].
-    iNext; iIntros "Hh". iDestruct (hinv_intro with "Hh Hlow") as "Hh".
-    iMod ("Hcl" with "* [Hh]") as "Ha"; first by eauto. by iApply "HΦ".
+    iApply (wp_load_big with "Hσ"); [done|exact: lookup_union_Some_l|].
+    iNext. iIntros "Hσ". iDestruct (hinv_intro with "Hσ Hlow Hlive") as "Hh".
+    iMod ("Hcl" with "* [Hh]") as "Hl"; first by eauto.
+    by iApply ("HΦ" with "[$Hl $HL]").
   Qed.
 
   Lemma wp_load_low p E l :
@@ -515,16 +650,15 @@ Section heap.
     {{{ heap_ctx ∗ ▷ low l }}} Load (Loc l) @ p; E
     {{{ v, RET v; low v }}}.
   Proof.
-    iIntros (? Φ) "[#Hinv >Hl] HΦ".
-    rewrite /heap_ctx low_loc lowloc'_eq /lowloc'_def.
-    iMod (auth_open_strong with "[$Hinv $Hl]")
-      as ([h h']) "(%&%&[Hh Hlow]&Hcl)"; first done.
+    iIntros (? Φ) "[Hh >Hl] HΦ". rewrite low_eq. iDestruct "Hl" as "[Hl HL]".
+    iMod (auth_open_strong with "[$Hh $Hl]")
+      as ([h h']) "(%&%&(Hσ & Hlow & Hlive)&Hcl)"; first done.
     case: (to_heap_low_included h h' l) => // ? [v ?].
-    iApply (wp_load_pst with "Hh"); [done|exact: lookup_union_Some_r'|].
-    iNext; iIntros "Hh".
+    iApply (wp_load_big with "Hσ"); [done|exact: lookup_union_Some_r'|].
+    iNext. iIntros "Hσ".
     iDestruct (big_sepM_lookup _ _ l v with "Hlow") as "#Hv"; first done.
-    iDestruct (hinv_intro with "Hh Hlow") as "Hh".
-    iMod ("Hcl" with "* [Hh]") as "Ha"; first by eauto.
+    iDestruct (hinv_intro with "Hσ Hlow Hlive") as "Hh".
+    iMod ("Hcl" with "* [Hh]") as "_"; first by eauto.
     by iApply ("HΦ" with "Hv").
   Qed.
 
@@ -533,15 +667,17 @@ Section heap.
     {{{ heap_ctx ∗ ▷ l ↦ v' }}} Store (Loc l) e @ p; E
     {{{ RET UnitV; l ↦ v }}}.
   Proof.
-    iIntros (<-%of_to_val ? Φ) "[#Hinv >Hl] HΦ".
-    rewrite /heap_ctx mapsto_eq /mapsto_def.
-    iMod (auth_open_strong with "[$Hinv $Hl]")
-      as ([h h']) "(%&%&[Hh Hlow]&Hcl)"; first done.
+    iIntros (<-%of_to_val ? Φ) "[Hh >Hl] HΦ".
+    rewrite high_eq. iDestruct "Hl" as "[Hl HL]".
+    iMod (auth_open_strong with "[$Hh $Hl]")
+      as ([h h']) "(%&%&(Hσ & Hlow & Hlive)&Hcl)"; first done.
     case: (to_heap_high_included h h' l 1 v') => // ??.
-    iApply (wp_store_pst with "Hh"); [done|exact: lookup_union_Some_l|].
-    iNext; iIntros "Hh". iDestruct (hinv_high with "Hh Hlow") as "Hh".
-    iMod ("Hcl" with "* [Hh]") as "Ha"; last by iApply "HΦ".
-    iFrame. iPureIntro. exact: to_heap_store_high.
+    iApply (wp_store_big with "Hσ"); [done|exact: lookup_union_Some_l|].
+    iDestruct (live_store_high _ _ l _ v with "Hlive") as "Hlive"=>//.
+    iNext. iIntros "Hσ". iDestruct (hinv_high with "Hσ Hlow Hlive") as "Hh".
+    iMod ("Hcl" with "* [Hh]") as "Hl".
+    - iFrame. iPureIntro. exact: to_heap_store_high.
+    - rewrite high_eq. by iApply ("HΦ" with "[$Hl $HL]").
   Qed.
 
   Lemma wp_store_low p E l e v :
@@ -549,15 +685,16 @@ Section heap.
     {{{ heap_ctx ∗ ▷ low  l ∗ ▷ low  v }}} Store (Loc l) e @ p; E
     {{{ RET UnitV; True }}}.
   Proof.
-    iIntros (<-%of_to_val ? Φ) "(#Hinv&>Hl&Hv) HΦ".
-    rewrite /heap_ctx low_loc lowloc'_eq /lowloc'_def.
-    iMod (auth_open_strong with "[$Hinv $Hl]")
-      as ([h h']) "(%&%&[Hh Hlow]&Hcl)"; first done.
+    iIntros (<-%of_to_val ? Φ) "(Hh&>Hl&Hv) HΦ".
+    rewrite low_eq. iDestruct "Hl" as "[Hl HL]".
+    iMod (auth_open_strong with "[$Hh $Hl]")
+      as ([h h']) "(%&%&(Hσ & Hlow & Hlive)&Hcl)"; first done.
     case: (to_heap_low_included h h' l) => // ? [v' ?].
-    iApply (wp_store_pst with "Hh"); [done|exact: lookup_union_Some_r'|].
-    iNext; iIntros "Hh".
-    iDestruct (hinv_store_low with "Hh Hlow Hv") as "Hh"; try done.
-    iMod ("Hcl" with "* [Hh]") as "Ha"; last by iApply "HΦ".
+    iApply (wp_store_big with "Hσ"); [done|exact: lookup_union_Some_r'|].
+    iDestruct (live_store_low _ _ _ _ v with "Hlive") as "Hlive"=>//.
+    iNext. iIntros "Hσ".
+    iDestruct (hinv_store_low with "Hv Hσ Hlow Hlive") as "Hh"; try done.
+    iMod ("Hcl" with "* [Hh]") as "_"; last by iApply "HΦ".
     iFrame. by erewrite to_heap_low_insert_override.
   Qed.
 
@@ -566,15 +703,16 @@ Section heap.
     {{{ heap_ctx ∗ ▷ l ↦{q} v' }}} CAS (Loc l) e1 e2 @ p; E
     {{{ RET LitV (LitBool false); l ↦{q} v' }}}.
   Proof.
-    iIntros (<-%of_to_val <-%of_to_val ?? Φ) "[#Hinv >Hl] HΦ".
-    rewrite /heap_ctx mapsto_eq /mapsto_def.
-    iMod (auth_open_strong with "[$Hinv $Hl]")
-      as ([h h']) "(%&%&[Hh Hlow]&Hcl)"; first done.
+    iIntros (<-%of_to_val <-%of_to_val ?? Φ) "[Hh >Hl] HΦ".
+    rewrite high_eq. iDestruct "Hl" as "[Hl HL]".
+    iMod (auth_open_strong with "[$Hh $Hl]")
+      as ([h h']) "(%&%&(Hσ & Hlow & Hlive)&Hcl)"; first done.
     case: (to_heap_high_included h h' l q v') => // ??.
-    iApply (wp_cas_fail_pst with "Hh");
+    iApply (wp_cas_fail_big with "Hσ");
       [done|exact: lookup_union_Some_l|done|].
-    iNext; iIntros "Hh". iDestruct (hinv_intro with "Hh Hlow") as "Hh".
-    iMod ("Hcl" with "* [Hh]") as "Ha"; first eauto. by iApply "HΦ".
+    iNext. iIntros "Hσ". iDestruct (hinv_intro with "Hσ Hlow Hlive") as "Hh".
+    iMod ("Hcl" with "* [Hh]") as "Hl".
+    by eauto. by iApply ("HΦ" with "[$Hl $HL]").
   Qed.
 
   Lemma wp_cas_suc p E l e1 v1 e2 v2 :
@@ -582,16 +720,18 @@ Section heap.
     {{{ heap_ctx ∗ ▷ l ↦ v1 }}} CAS (Loc l) e1 e2 @ p; E
     {{{ RET LitV (LitBool true); l ↦ v2 }}}.
   Proof.
-    iIntros (<-%of_to_val <-%of_to_val ? Φ) "[#Hinv >Hl] HΦ".
-    rewrite /heap_ctx mapsto_eq /mapsto_def.
-    iMod (auth_open_strong with "[$Hinv $Hl]")
-      as ([h h']) "(%&%&[Hh Hlow]&Hcl)"; first done.
+    iIntros (<-%of_to_val <-%of_to_val ? Φ) "[Hh >Hl] HΦ".
+    rewrite high_eq. iDestruct "Hl" as "[Hl HL]".
+    iMod (auth_open_strong with "[$Hh $Hl]")
+      as ([h h']) "(%&%&(Hσ & Hlow & Hlive)&Hcl)"; first done.
     case: (to_heap_high_included h h' l 1 v1) => // ??.
-    iApply (wp_cas_suc_pst with "Hh");
+    iDestruct (live_store_high _ _ l _ v2 with "Hlive") as "Hlive"=>//.
+    iApply (wp_cas_suc_big with "Hσ");
       [done|exact: lookup_union_Some_l|].
-    iNext; iIntros "Hh". iDestruct (hinv_high with "Hh Hlow") as "Hh".
-    iMod ("Hcl" with "* [Hh]") as "Ha"; last by iApply "HΦ".
-    iFrame. iPureIntro. exact: to_heap_store_high.
+    iNext. iIntros "Hσ". iDestruct (hinv_high with "Hσ Hlow Hlive") as "Hh".
+    iMod ("Hcl" with "* [Hh]") as "Hl".
+    - iFrame. iPureIntro. exact: to_heap_store_high.
+    - rewrite high_eq. by iApply ("HΦ" with "[$Hl $HL]").
   Qed.
 
   Lemma wp_cas_low p E l e1 v1 e2 v2 :
@@ -599,34 +739,71 @@ Section heap.
     {{{ heap_ctx ∗ ▷ low l ∗ ▷ low v2 }}} CAS (Loc l) e1 e2 @ p; E
     {{{ b, RET LitV (LitBool b); True }}}.
   Proof.
-    iIntros (<-%of_to_val <-%of_to_val ? Φ) "(#Hinv&>Hl&Hv) HΦ".
-    rewrite /heap_ctx low_loc lowloc'_eq /lowloc'_def.
-    iMod (auth_open_strong with "[$Hinv $Hl]")
-      as ([h h']) "(%&%&[Hh Hlow]&Hcl)"; first done.
+    iIntros (<-%of_to_val <-%of_to_val ? Φ) "(Hh&>Hl&Hv) HΦ".
+    rewrite low_eq. iDestruct "Hl" as "[Hl HL]".
+    iMod (auth_open_strong with "[$Hh $Hl]")
+      as ([h h']) "(%&%&(Hσ & Hlow & Hlive)&Hcl)"; first done.
     case: (to_heap_low_included h h' l) => // ? [v' ?].
     case: (decide (v' = v1)) => [<-|?].
-    - iApply (wp_cas_suc_pst with "Hh");
+    - iApply (wp_cas_suc_big with "Hσ");
         [done|exact: lookup_union_Some_r'|].
-      iNext; iIntros "Hh".
-      iDestruct (hinv_store_low with "Hh Hlow Hv") as "Hh"; try done.
-      iMod ("Hcl" with "* [Hh]") as "Ha"; last by iApply "HΦ".
+      iNext. iIntros "Hσ".
+      iDestruct (live_store_low _ _ _ _ v2 with "Hlive") as "Hlive"=>//.
+      iDestruct (hinv_store_low with "Hv Hσ Hlow Hlive") as "Hh"; try done.
+      iMod ("Hcl" with "* [Hh]") as "_"; last by iApply "HΦ".
       iFrame. by erewrite to_heap_low_insert_override.
-    - iApply (wp_cas_fail_pst with "Hh");
+    - iApply (wp_cas_fail_big with "Hσ");
         [done|exact: lookup_union_Some_r'|done|].
-      iNext; iIntros "Hh". iDestruct (hinv_intro with "Hh Hlow") as "Hh".
-      iMod ("Hcl" with "* [Hh]") as "Ha"; first by eauto. by iApply "HΦ".
+      iNext. iIntros "Hσ". iDestruct (hinv_intro with "Hσ Hlow Hlive") as "Hh".
+      iMod ("Hcl" with "* [Hh]") as "_". by eauto. by iApply "HΦ".
   Qed.
 End heap.
+Typeclasses Opaque liveloc' mapsto lowloc' heap_ctx'.
 
-(**
-	By the heap invariant, we can always inspect or modify the
-	heap on low values.
-*)
-Section wp_low_val.
+(** ** Derived rules *)
+Section derived.
   Context `{heapG Σ}.
   Implicit Types e : expr.
   Implicit Types v : val.
 
+  (**
+	We can allocate high and low locations, observing
+	freshness or not.
+  *)
+  Lemma wp_alloc p E e v :
+    to_val e = Some v → ↑heapN ⊆ E →
+    {{{ heap_ctx }}} Alloc e @ p; E {{{ l, RET LocV l; l ↦ v }}}.
+  Proof.
+    iIntros (?? Φ) "Hh HΦ".
+    iApply (wp_alloc_live _ _ _ _ ∅ with "[$Hh]"); eauto;
+      first by rewrite /live big_sepS_empty.
+    iNext. iIntros (l) "[Hl _]". by iApply "HΦ".
+  Qed.
+
+  Lemma wp_alloc_low_live p E e v X :
+    to_val e = Some v → ↑heapN ⊆ E →
+    {{{ heap_ctx ∗ ▷ low v ∗ live X }}} Alloc e @ p; E
+    {{{ l, RET LocV l; low l ∗ ⌜l ∉ X⌝ }}}.
+  Proof.
+    iIntros (?? Φ) "(#Hh & Hv & HX) HΦ". rewrite -wp_fupd.
+    iApply (wp_alloc_live with "[$Hh $HX]"); eauto. iNext.
+    iIntros (l) "(Hl & HX)". rewrite [(l ↦ v)%I]later_intro [low _]later_intro.
+    iMod (heap_mark_low with "Hh Hl Hv") as "Hl"; first done.
+    by iApply ("HΦ" with "[$Hl $HX]").
+  Qed.
+
+  Lemma wp_alloc_low p E e v :
+    to_val e = Some v → ↑heapN ⊆ E →
+    {{{ heap_ctx ∗ ▷ low v }}} Alloc e @ p; E
+    {{{ l, RET LocV l; low l }}}.
+  Proof.
+    iIntros (?? Φ) "(Hh & Hv) HΦ".
+    iApply (wp_alloc_low_live _ _ _ _ ∅ with "[$Hh $Hv]"); eauto;
+      first by rewrite /live big_sepS_empty.
+    iNext. iIntros (l) "[Hl _]". by iApply "HΦ".
+  Qed.
+
+  (** We can always eliminate low values. *)
   Lemma wp_low_alloc E e :
     ↑heapN ⊆ E →
     heap_ctx -∗
@@ -677,4 +854,4 @@ Section wp_low_val.
     iApply (wp_cas_low with "[$Hh Hl0 Hv2]"); try auto.
     iNext. iIntros. by simpl_on_val.
   Qed.
-End wp_low_val.
+End derived.
